CommonST.v
@@ -1,5 +1,5 @@
-Require Import TraceModel. 
-Require Import Properties.
+Require Import TraceModel2. 
+Require Import Properties2.
 Require Import ClassicalExtras.
 
 Set Implicit Arguments. 
@@ -120,6 +120,6 @@ Definition determinacy (K : level) : Prop :=
 
 Definition semantics_safety_like (K : level) : Prop :=
   forall t P,
-    ~ sem K P t -> inf t ->
+    ~ sem K P t -> inf t -> ~ diverges t ->
     (exists m ebad, psem P m /\ prefix (fsnoc m ebad) t /\ ~ psem P (fsnoc m ebad)).
 
